PREFIX : <https://linked.data.gov.au/def/rct/>
PREFIX cs: <https://linked.data.gov.au/def/rct>
PREFIX dcterms: <http://purl.org/dc/terms/>
PREFIX rdfs: <http://www.w3.org/2000/01/rdf-schema#>
PREFIX sdo: <https://schema.org/>
PREFIX reg: <http://purl.org/linked-data/registry#>
PREFIX skos: <http://www.w3.org/2004/02/skos/core#>
PREFIX status: <http://def.isotc211.org/iso19135/-1/2015/CoreModel/code/RE_ItemStatus/>
PREFIX xsd: <http://www.w3.org/2001/XMLSchema#>

cs:
    a skos:ConceptScheme ;
    dcterms:created "2023-05-16"^^xsd:date ;
    dcterms:creator <https://linked.data.gov.au/org/qsi> ;
    dcterms:issued "2023-05-16"^^xsd:date ;
    dcterms:license "https://creativecommons.org/licenses/by/4.0/"^^xsd:anyURI ;
    dcterms:modified "2023-05-16"^^xsd:date ;
    dcterms:publisher <https://linked.data.gov.au/org/qsi> ;
    dcterms:rights "(c) The State of Queensland (Department of Resources), 2023" ;
    dcterms:source "https://linked.data.gov.au/def/roads"^^xsd:anyURI ;
    reg:status status:stable ;
    skos:definition "Types of Feature C=Label Component used to characterise roads (street)' labels'"@en ;
    skos:hasTopConcept
        :roadPrefix ,
        :roadName ,
        :roadType ,
        :roadSuffix ;
    skos:prefLabel "Feature Label Component Types for Roads"@en ;
    skos:scopeNote "This vocabulary may be extended if road names are found to be better represented by more/other component types."
.

<https://linked.data.gov.au/org/qsi>
    a sdo:Organization ;
    sdo:description "The unit within Queensland Government that manages fundamental spatial information for the State."@en ;
    sdo:name "Queensland Spatial Information" ;
    sdo:url "https://qldspatial.information.qld.gov.au"^^xsd:anyURI ;
.

:roadPrefix
    a skos:Concept ;
    dcterms:provenance "Created for Queensland Spatial Information's Cadastre & Address Model project, 2023"@en ;
    rdfs:isDefinedBy cs: ;
    reg:status status:original ;
    skos:definition "A literal initial part of a road's label that comes before the road's name"@en ;
    skos:inScheme cs: ;
    skos:prefLabel "Road Prefix"@en ;
.

:roadName
    a skos:Concept ;
    dcterms:provenance "Created for Queensland Spatial Information's Cadastre & Address Model project, 2023"@en ;
    rdfs:isDefinedBy cs: ;
    reg:status status:original ;
    skos:definition "The literal name of the road, without any expression of the road's type"@en ;
    skos:inScheme cs: ;
    skos:prefLabel "Road Name"@en ;
.

:roadType
    a skos:Concept ;
    dcterms:provenance "Created for Queensland Spatial Information's Cadastre & Address Model project, 2023"@en ;
    rdfs:isDefinedBy cs: ;
    reg:status status:original ;
    skos:definition "A reference to the type of the road, selected from a controlled list of road (street) types"@en ;
    skos:inScheme cs: ;
    skos:prefLabel "Road Type"@en ;
.

:roadSuffix
    a skos:Concept ;
    dcterms:provenance "Created for Queensland Spatial Information's Cadastre & Address Model project, 2023"@en ;
    reg:status status:original ;
    rdfs:isDefinedBy cs: ;
    skos:definition "A literal initial part of a road's label that comes after the road's name and type value"@en ;
    skos:inScheme cs: ;
    skos:prefLabel "Road Suffix"@en ;
.
